src/frontends/lean/parser.h
@@ -165,6 +165,7 @@ class parser : public abstract_parser {
     std::shared_ptr<snapshot> mk_snapshot();
 
     friend class module_parser;
+    friend class patexpr_to_expr_fn;
 
 public:
     parser(environment const & env, io_state const & ios,
@@ -351,7 +352,7 @@ public:
     void parse_close_binder_info(binder_info const & bi) { return parse_close_binder_info(optional<binder_info>(bi)); }
 
     /** \brief Convert an identifier into an expression (constant or local constant) based on the current scope */
-    expr id_to_expr(name const & id, pos_info const & p, bool resolve_only = false);
+    expr id_to_expr(name const & id, pos_info const & p, bool resolve_only = false, list<name> const & extra_locals = list<name>());
 
     expr parse_expr(unsigned rbp = 0);
     /** \brief Parse an (optionally) qualified expression.
