library/data/buffer.lean
@@ -22,67 +22,67 @@ mk_buffer
 def size (b : buffer α) : nat :=
 b.1
 
-def to_array (b : buffer α) : array α (b^.size) :=
+def to_array (b : buffer α) : array α (b.size) :=
 b.2
 
 def push_back : buffer α → α → buffer α
-| ⟨n, a⟩ v := ⟨n+1, a^.push_back v⟩
+| ⟨n, a⟩ v := ⟨n+1, a.push_back v⟩
 
 def pop_back : buffer α → buffer α
 | ⟨0, a⟩   := ⟨0, a⟩
-| ⟨n+1, a⟩ := ⟨n, a^.pop_back⟩
+| ⟨n+1, a⟩ := ⟨n, a.pop_back⟩
 
-def read : Π (b : buffer α), fin b^.size → α
-| ⟨n, a⟩ i := a^.read i
+def read : Π (b : buffer α), fin b.size → α
+| ⟨n, a⟩ i := a.read i
 
-def write : Π (b : buffer α), fin b^.size → α → buffer α
-| ⟨n, a⟩ i v := ⟨n, a^.write i v⟩
+def write : Π (b : buffer α), fin b.size → α → buffer α
+| ⟨n, a⟩ i v := ⟨n, a.write i v⟩
 
 def read' [inhabited α] : buffer α → nat → α
-| ⟨n, a⟩ i := a^.read' i
+| ⟨n, a⟩ i := a.read' i
 
 def write' : buffer α → nat → α → buffer α
-| ⟨n, a⟩ i v := ⟨n, a^.write' i v⟩
+| ⟨n, a⟩ i v := ⟨n, a.write' i v⟩
 
 def to_list (b : buffer α) : list α :=
-b^.to_array^.to_list
+b.to_array.to_list
 
 protected def to_string (b : buffer α) : list α :=
-b^.to_array^.to_list^.reverse
+b.to_array.to_list.reverse
 
 def append_list {α : Type u} : buffer α → list α → buffer α
 | b []      := b
-| b (v::vs) := append_list (b^.push_back v) vs
+| b (v::vs) := append_list (b.push_back v) vs
 
 def append_string (b : buffer char) (s : string) : buffer char :=
-b^.append_list s^.reverse
+b.append_list s.reverse
 
 def append_array {α : Type u} {n : nat} (nz : n > 0) : buffer α → array α n → ∀ i : nat, i < n → buffer α
 | ⟨m, b⟩ a 0     _ :=
   let i : fin n := ⟨n - 1, array.lt_aux_2 nz⟩ in
-  ⟨m+1, b^.push_back (a^.read i)⟩
+  ⟨m+1, b.push_back (a.read i)⟩
 | ⟨m, b⟩ a (j+1) h :=
   let i : fin n := ⟨n - 2 - j, array.lt_aux_3 h⟩ in
-  append_array ⟨m+1, b^.push_back (a^.read i)⟩ a j (array.lt_aux_1 h)
+  append_array ⟨m+1, b.push_back (a.read i)⟩ a j (array.lt_aux_1 h)
 
 protected def append {α : Type u} : buffer α → buffer α → buffer α
 | b ⟨0, a⟩   := b
 | b ⟨n+1, a⟩ := append_array (nat.zero_lt_succ _) b a n (nat.lt_succ_self _)
 
-def iterate : Π b : buffer α, β → (fin b^.size → α → β → β) → β
-| ⟨_, a⟩ b f := a^.iterate b f
+def iterate : Π b : buffer α, β → (fin b.size → α → β → β) → β
+| ⟨_, a⟩ b f := a.iterate b f
 
-def foreach : Π b : buffer α, (fin b^.size → α → α) → buffer α
-| ⟨n, a⟩ f := ⟨n, a^.foreach f⟩
+def foreach : Π b : buffer α, (fin b.size → α → α) → buffer α
+| ⟨n, a⟩ f := ⟨n, a.foreach f⟩
 
 def map (f : α → α) : buffer α → buffer α
-| ⟨n, a⟩ := ⟨n, a^.map f⟩
+| ⟨n, a⟩ := ⟨n, a.map f⟩
 
 def foldl : buffer α → β → (α → β → β) → β
-| ⟨_, a⟩ b f := a^.foldl b f
+| ⟨_, a⟩ b f := a.foldl b f
 
-def rev_iterate : Π (b : buffer α), β → (fin b^.size → α → β → β) → β
-| ⟨_, a⟩ b f := a^.rev_iterate b f
+def rev_iterate : Π (b : buffer α), β → (fin b.size → α → β → β) → β
+| ⟨_, a⟩ b f := a.rev_iterate b f
 
 instance : has_append (buffer α) :=
 ⟨buffer.append⟩
@@ -99,6 +99,6 @@ meta instance [has_to_tactic_format α] : has_to_tactic_format (buffer α) :=
 end buffer
 
 def list.to_buffer {α : Type u} (l : list α) : buffer α :=
-mk_buffer^.append_list l
+mk_buffer.append_list l
 
 @[reducible] def char_buffer := buffer char
